theories/BWT/Sorting/Key.v
@@ -1,5 +1,6 @@
 Require Import Coq.Lists.List.
 Require Import Coq.omega.Omega.
+Require Import Coq.Sorting.Permutation.
 
 Require Import BWT.Sorting.InsertionSort.
 Require Import BWT.Sorting.Lexicographic.
@@ -8,13 +9,13 @@ Require Import BWT.Sorting.Sorted.
 Require Import BWT.Lib.List.
 
 Section KeyOrd.
-  Context {A K : Type} `{O: Ord K}.
+  Context {A K : Type} `{O: Preord K}.
 
   Variable key : A -> K.
 
-  Definition keyOrd : Ord A.
+  Definition keyOrd : Preord A.
   Proof.
-    apply Build_Ord with (le := fun x y => le (key x) (key y));
+    apply Build_Preord with (le := fun x y => le (key x) (key y));
       intros; eauto using le_trans, le_total, le_dec.
   Defined.
 
@@ -68,7 +69,7 @@ Section KeyOrd.
 End KeyOrd.
 
 Section Firstn.
-  Context {A : Type} {O: Ord A}.
+  Context {A : Type} {O: Preord A}.
 
   Local Arguments le {_} _.
   Local Arguments lt {_} _.
@@ -116,7 +117,7 @@ Section Firstn.
     unfold eqv. intuition.
   Qed.
 
-  Theorem key_le_firstn_gt : forall j x y,
+  Theorem key_le_firstn_S : forall j x y,
       le (keyOrd (firstn (S j))) x y ->
       le (keyOrd (firstn j)) x y.
   Proof.
@@ -124,59 +125,58 @@ Section Firstn.
     rewrite key_le in *.
     apply lt_spec in H.
     destruct H.
-    apply lex_lt_destr in H.
-    destruct H as [hx [tx [hy [ty [Hx [Hy [Hlt Heq]]]]]]].
-    remember (length hx) as n.
-    assert (Heqn' : n = length hy). {
-      apply lex_eqv_iff in Heq.
-      subst n. eapply Forall2_length; eauto.
-    }
-    destruct (Nat.le_gt_cases (S j) n).
-    + assert (HT: tx = nil /\ ty = nil). {
-        apply f_equal with (f := @length A) in Hx; apply f_equal with (f := @length A) in Hy.
-        rewrite app_length in *.
-        rewrite <- Heqn in Hx. rewrite <- Heqn' in Hy.
-        pose proof (firstn_le_length (S j) x).
-        pose proof (firstn_le_length (S j) y).
-        split; apply length_zero_iff_nil; omega.
+    + apply lex_lt_destr in H.
+      destruct H as [hx [tx [hy [ty [a [Hx [Hy [Hlt Heq]]]]]]]].
+      remember (length hx) as n.
+      assert (Heqn' : n = length hy). {
+        apply lex_eqv_iff in Heq.
+        subst n. eapply Forall2_length; eauto.
       }
-      destruct HT; subst tx ty.
-      rewrite app_nil_r in *.
-      apply f_equal with (f := firstn j) in Hx; apply f_equal with (f := firstn j) in Hy.
-      rewrite firstn_firstn in *.
-      replace (Nat.min j (S j)) with j in * by (symmetry; apply Nat.min_l; omega).
-      rewrite Hx, Hy.
-      apply lex_eqv_firstn. symmetry. auto.
-    +
-      pose proof (firstn_le_length (S j) x).
-      rewrite firstn_all2 in Hx.
+      destruct (Nat.le_gt_cases (S j) n).
+      * assert (HT: tx = nil /\ (a :: ty) = nil). {
+          apply f_equal with (f := @length A) in Hx; apply f_equal with (f := @length A) in Hy.
+          rewrite app_length in *.
+          rewrite <- Heqn in Hx. rewrite <- Heqn' in Hy.
+          pose proof (firstn_le_length (S j) x).
+          pose proof (firstn_le_length (S j) y).
+          cbn [length] in Hy.
+          split; apply length_zero_iff_nil; omega.
+        }
+        destruct HT. discriminate.
+      * assert (HLE : n <= j) by omega.
+        apply Nat.le_exists_sub in HLE.
+        destruct HLE as [p [HP _]].
+        apply f_equal with (f := firstn j) in Hx; apply f_equal with (f := firstn j) in Hy.
+        rewrite firstn_firstn in *.
+        replace (Nat.min j (S j)) with j in * by (symmetry; apply Nat.min_l; omega).
+        rewrite plus_comm in HP.
+        rewrite HP in Hx at 2, Hy at 2; rewrite Heqn in Hx; rewrite Heqn' in Hy.
+        rewrite firstn_app_2 in Hx, Hy.
+        rewrite Hx, Hy.
+        apply lex_eqv_prepend; auto.
+        destruct p; [rewrite firstn_O; apply lex_le_nil|].
+        apply lex_lt_iff in Hlt.
+        inversion Hlt; subst; clear Hlt.
+        rewrite firstn_nil; apply lex_le_nil.
+        apply lex_le_cons_lt; auto.
+        inversion H4.
+    + assert (HLJ : forall l : list A, firstn j l = firstn j (firstn (S j) l)). {
+        intros l.
+        rewrite firstn_firstn.
+        replace (Nat.min j (S j)) with j by (symmetry; apply Nat.min_l; omega).
+        reflexivity.
+      }
+      assert (HE: eqv List_Lex_Preord (firstn j x) (firstn j y)). {
+        rewrite (HLJ x), (HLJ y).
+        apply lex_eqv_firstn.
+        auto.
+      }
+      destruct HE as [HE _].
+      auto.
+  Qed.
 
-
-
-    destruct x as [|a x]; [rewrite firstn_nil; constructor|].
-    destruct y as [|b y]; [symmetry in Hy; apply app_eq_nil in Hy; destruct Hy; subst; apply lex_lt_iff in Hlt; inversion Hlt|].
-    cbn in Hx; cbn in Hy.
-    destruct hx as [|hxhd hxtl].
-    replace hy with (@nil A) in * by (apply lex_eqv_iff in Heq; inversion Heq; auto).
-
-
-
-    cbn in Hx.
-    rewrite key_le.
-    destruct (Nat.lt_ge_cases (S j))
-    Search "<".
-    destruct ()
-
-    pose proof (lex_)
-    rewrite key_le in H.
-    destruct (Nat.le_gt_cases (length x) (S j)).
-    - rewrite firstn_all2 in H by omega.
-
-      r
-        ewrite firstn_length_le in H.
-
-  Theorem key_le_firstn_gt : forall k j x y,
-      j < k ->
+  Theorem key_le_firstn_ge : forall k j x y,
+      j <= k ->
       le (keyOrd (firstn k)) x y ->
       le (keyOrd (firstn j)) x y.
   Proof.
@@ -186,9 +186,9 @@ Section Firstn.
     - apply le_lt_or_eq in HJK.
       destruct HJK.
       apply IHk. omega.
-      admit.
-      inversion H; subst.
-
+      apply key_le_firstn_S. auto.
+      rewrite H. auto.
+  Qed.
 
   Theorem key_firstn_S : forall n x y,
       le (keyOrd (firstn 1)) x y ->
@@ -205,8 +205,42 @@ Section Firstn.
       apply key_lt_firstn_1 in HLt. auto.
     - apply lex_le_cons_eq.
       apply key_eqv_firstn_1 in HEq. auto.
-      apply IHn. cbn in Ln. app
+      cbn [tl] in Ln. apply Ln.
+  Qed.
 
+  Theorem key_lt_firstn_S : forall j x y,
+      lt (keyOrd (firstn j)) x y ->
+      lt (keyOrd (firstn (S j))) x y.
+  Proof.
+    induction j; intros x y HLT; apply lex_lt_iff in HLT; apply lex_lt_iff.
+    - rewrite !firstn_O in HLT.
+      inversion HLT.
+    - remember (S j) as j'.
+      destruct x as [|hx tx]; (destruct y as [|hy ty]; [rewrite firstn_nil in HLT; inversion HLT|]).
+      + apply lex_lt_nil.
+      + rewrite Heqj', !firstn_cons in HLT.
+        inversion HLT; subst x y xs ys; clear HLT.
+        * apply lex_lt_cons_lt; auto.
+        * rewrite !firstn_cons.
+          apply lex_lt_cons_eq; auto.
+          subst j'.
+          apply lex_lt_iff; apply IHj.
+          apply lex_lt_iff; auto.
+  Qed.
+
+  Theorem key_lt_firstn_ge : forall k j x y,
+      j <= k ->
+      lt (keyOrd (firstn j)) x y ->
+      lt (keyOrd (firstn k)) x y.
+  Proof.
+    induction k; intros j x y HJK HLtK.
+    - assert (j = 0) by omega.
+      subst j. apply lex_lt_iff in HLtK. inversion HLtK.
+    - apply le_lt_or_eq in HJK.
+      destruct HJK.
+      apply key_lt_firstn_S. apply (IHk j); [omega|auto].
+      rewrite <- H. auto.
+  Qed.
 End Firstn.
 
 Section HdSort.
@@ -218,7 +252,7 @@ Section HdSort.
 End HdSort.
 
 Section Prefix.
-  Context {A : Type} `{O: Ord A}.
+  Context {A : Type} `{O: Preord A}.
 
   Local Arguments Sorted {_} _ _.
 
@@ -231,6 +265,76 @@ Section Prefix.
     intros l. unfold PrefixSorted.
     induction l; [apply Sorted_nil|].
     apply Sorted_cons.
-    intros. apply key_firstn_O. apply IHl.
+    intros. apply key_le_firstn_O. apply IHl.
   Qed.
 End Prefix.
+
+Section Insert.
+  Context {A : Type} {P : Preord A} {O : @Ord A P}.
+
+  Local Arguments eqv {_} _.
+  Local Arguments le {_} _.
+  Local Arguments le_dec {_} _.
+  Local Arguments lt {_} _.
+  Local Arguments tl {_}.
+  Local Arguments Sorted {_}.
+  Local Arguments insert {_}.
+  Local Arguments sort {_}.
+
+  Theorem insert_sorted_S : forall colmat' colmat a n,
+      PrefixSorted (S n) colmat' ->
+      Permutation colmat colmat' ->
+      PrefixSorted n (tl a :: map tl colmat) ->
+      PrefixSorted (S n) (insert (keyOrd (firstn 1)) a colmat').
+  Proof.
+    induction colmat' as [|b colmat']; intros colmat a n HS' HP HS.
+    apply Sorted_1.
+    cbn [insert]. destruct (le_dec (keyOrd (firstn 1)) a b).
+    - apply Sorted_LocallySorted_iff.
+      constructor. apply Sorted_LocallySorted_iff.
+      apply HS'. apply key_firstn_S; [auto|].
+      apply Sorted_cons_inv in HS; destruct HS as [HLe HS].
+      apply HLe. apply in_map. eapply Permutation_in. symmetry. apply HP.
+      left; auto.
+    - assert (PrefixSorted (S n) (insert (keyOrd (firstn 1)) a colmat')). {
+        assert (In b colmat). eapply Permutation_in; [symmetry; apply HP|left; auto].
+        apply rem1_in_split in H.
+        destruct H as [l1 [l2 [Hcolmat Hcolmatrem]]].
+        apply IHcolmat' with (colmat := l1 ++ l2).
+        apply Sorted_cons_inv in HS'; destruct HS'. auto.
+        symmetry in HP. apply Permutation_rem1 in HP.
+        symmetry. rewrite <- Hcolmatrem. auto.
+        rewrite <- Hcolmatrem.
+        apply Sorted_cons_inv in HS; destruct HS as [HLe HS].
+        apply Sorted_cons.
+        intros. apply HLe. rewrite rem1_map in H. apply in_rem1_in in H.
+        auto.
+        rewrite !rem1_map.
+        apply Sorted_rem1. auto.
+      }
+      clear IHcolmat'.
+      apply Sorted_cons.
+      + intros x HIn.
+        apply Permutation_in with (l' := a :: colmat') in HIn; [|symmetry; apply insert_perm].
+        destruct HIn.
+        * subst.
+          apply lt_le.
+          apply key_lt_firstn_ge with (j := 1); [omega|].
+          auto.
+        * apply Sorted_cons_inv in HS'; destruct HS' as [HLe _].
+          apply HLe. auto.
+      + auto.
+  Qed.
+
+  Theorem sort_sorted_S : forall (colmat : list (list A)) n,
+    PrefixSorted n (map tl colmat) ->
+    PrefixSorted (S n) (sort (keyOrd (firstn 1)) colmat).
+  Proof.
+    induction colmat; intros n HS; [constructor|].
+    cbn [map sort].
+    eapply insert_sorted_S.
+    + apply IHcolmat. inversion HS; auto.
+    + apply sort_perm.
+    + auto.
+  Qed.
+End Insert.
