theories/BWT/Sorting/Ord.v
@@ -4,87 +4,106 @@ Require Import Coq.Classes.RelationClasses.
 Require Import Coq.Program.Basics.
 Require Import Coq.Relations.Relation_Definitions.
 Require Import Coq.Setoids.Setoid.
+Require Import Coq.Classes.EquivDec.
 
-(** A type equipped with a total, decidable preorder. *)
-
-Class Ord (A : Type):=
+Class Preord (A : Type) :=
   { le : A -> A -> Prop;
     le_trans : forall x y z, le x y -> le y z -> le x z;
     le_total : forall x y, le x y \/ le y x;
     le_dec : forall x y, {le x y} + {~le x y};
   }.
 
-Lemma le_refl {A} `{Ord A} : forall x, le x x.
+Lemma le_refl `{Preord} : forall x, le x x.
 Proof.
   intros. destruct (le_total x x); auto.
 Qed.
 
-Lemma le_not {A} `{Ord A} : forall x y, ~(le x y) -> le y x.
-Proof.
-  intros. destruct (le_total x y). contradiction. auto.
-Qed.
+Add Parametric Relation (A : Type) `(Preord A) : A le
+    reflexivity proved by le_refl
+    transitivity proved by le_trans
+      as preord_le_rel.
 
-Definition le_decb {A} `{Ord A} x y := proj1_sig (bool_of_sumbool (le_dec x y)).
+Section Preord.
+  Context {A : Type} {O : Preord A}.
 
-Definition ge {A} `{Ord A} x y := le y x.
-Definition lt {A} `{Ord A} x y := ~ (le y x).
-Definition gt {A} `{Ord A} x y := ~ (le x y).
+  Definition ge x y := le y x.
+  Definition lt x y := ~ (le y x).
+  Definition gt x y := ~ (le x y).
 
-(** Two elements are equivalent if they compare [le] in both directions. *)
-
-Definition eqv {A} `{Ord A} (x y : A) : Prop := le x y /\ le y x.
-
-Program Definition eqv_dec {A} `{Ord A} (x y : A) : {eqv x y} + {~ eqv x y} :=
-  if le_dec x y then
-    if le_dec y x then left _
-    else right _
-  else right _.
-Solve All Obligations with unfold eqv; intuition eauto.
-
-Definition eqv_decb {A} `{Ord A} x y := proj1_sig (bool_of_sumbool (eqv_dec x y)).
-
-Section Equiv.
-  Context {A} `{Ord A}.
-
-  Theorem eqv_refl : forall x, eqv x x.
+  Lemma lt_le_rev : forall x y, lt y x -> le y x.
   Proof.
-    intros.
-    unfold eqv. split; apply le_refl.
+    intros. destruct (le_total x y). contradiction. auto.
   Qed.
 
-  Theorem eqv_sym : forall x y, eqv x y -> eqv y x.
-  Proof. intros. unfold eqv in *. intuition. Qed.
+  Definition le_decb x y := proj1_sig (bool_of_sumbool (le_dec x y)).
+End Preord.
 
-  Theorem eqv_trans : forall x y z , eqv x y -> eqv y z -> eqv x z.
-  Proof. intros. unfold eqv in *. intuition (eapply le_trans; eauto). Qed.
+Definition eqv `{Preord} x y := le x y /\ le y x.
 
-  (* Instance Equivalence_eqv : Equivalence eqv | 0 := *)
-  (*   { Equivalence_Reflexive := eqv_refl; *)
-  (*     Equivalence_Symmetric := eqv_sym; *)
-  (*     Equivalence_Transitive := eqv_trans; *)
-  (*   }. *)
+Theorem eqv_refl `{Preord} : forall x, eqv x x.
+Proof.
+  intros. unfold eqv. split; reflexivity.
+Qed.
+
+Theorem eqv_sym `{Preord} : forall x y, eqv x y -> eqv y x.
+Proof. intros. unfold eqv in *. intuition. Qed.
+
+Theorem eqv_trans `{Preord} : forall x y z , eqv x y -> eqv y z -> eqv x z.
+Proof. intros. unfold eqv in *. intuition (eapply le_trans; eauto). Qed.
+
+Add Parametric Relation (A : Type) `(Preord A) : A eqv
+    reflexivity proved by eqv_refl
+    symmetry proved by eqv_sym
+    transitivity proved by eqv_trans
+      as eqv_rel.
+
+Add Parametric Morphism `(Preord) : le with
+      signature eqv ==> eqv ==> iff as le_mor.
+Proof.
+  intros.
+  unfold eqv in *. intuition; eauto using le_trans.
+Qed.
+
+Add Parametric Morphism `(Preord): lt with
+      signature eqv ==> eqv ==> iff as lt_mor.
+Proof.
+  intros.
+  unfold eqv, lt in *. intuition; eauto using le_trans.
+Qed.
+
+Section Eqv.
+  Context {A : Type} {O : Preord A}.
+
+  Program Definition eqv_dec x y : {eqv x y} + {~ eqv x y} :=
+    if le_dec x y then
+      if le_dec y x then left _
+      else right _
+    else right _.
+  Solve All Obligations with unfold eqv; intuition eauto.
+
+  Definition eqv_decb x y := proj1_sig (bool_of_sumbool (eqv_dec x y)).
 
   Theorem eqv_def : forall x y,
       eqv x y <-> (le x y /\ le y x).
   Proof. reflexivity. Qed.
 
-  (* Instance EqDec_eqv : EqDec A eqv | 0 := eqv_dec. *)
-
-  Theorem eqv_subst : forall x y z, eqv x y -> (eqv x z <-> eqv y z).
-  Proof.
-    intros.
-    repeat rewrite eqv_def in *.
-    intuition; eauto using le_trans.
-  Qed.
-End Equiv.
+  Global Instance Preord_eqv_Equivalence : Equivalence eqv := {}.
+  Global Instance Ord_EqDec : EqDec A eqv := eqv_dec.
+End Eqv.
 
 Section Lt.
-  Context {A} `{Ord A}.
+  Context {A : Type} {O : Preord A}.
 
   Theorem lt_spec : forall x y, le x y <-> lt x y \/ eqv x y.
   Proof.
     intros.
-    destruct (eqv_dec x y); unfold lt, eqv in *; intuition; eauto using le_not.
+    destruct (eqv_dec x y); unfold lt, eqv in *; intuition; eauto using lt_le_rev.
+  Qed.
+
+  Theorem lt_spec2 : forall x y, lt x y <-> le x y /\ ~ eqv x y.
+  Proof.
+    intros.
+    destruct (eqv_dec x y); unfold lt, eqv in *; intuition; eauto using lt_le_rev.
   Qed.
 
   Program Definition lt_eq_dec x y : {lt x y} + {eqv x y} + {lt y x} :=
@@ -103,7 +122,7 @@ Section Lt.
   Theorem lt_trans : forall x y z, lt x y -> lt y z -> lt x z.
   Proof.
     intros. unfold lt in *.
-    match goal with [ H : ~ le _ _ |- _ ] => apply le_not in H end.
+    match goal with [ H : ~ le _ _ |- _ ] => apply lt_le_rev in H end.
     intro.
     eauto using le_trans.
   Qed.
@@ -118,26 +137,18 @@ Section Lt.
   Proof. unfold lt, eqv in *. intuition. Qed.
 
   Theorem lt_le : forall x y, lt x y -> le x y.
-  Proof. unfold lt. intros. apply le_not. auto. Qed.
-
+  Proof. unfold lt. intros. apply lt_le_rev. auto. Qed.
 End Lt.
 
-Add Parametric Relation {A} `{Ord A} : A eqv
-    reflexivity proved by eqv_refl
-    symmetry proved by eqv_sym
-    transitivity proved by eqv_trans
-  as eqv_rel.
+Section Ord.
+  Class Ord (A : Type) `{Preord A} :=
+    { eqv_eq : forall x y, eqv x y -> x = y }.
 
-Add Parametric Morphism {A} `{Ord A} : le with
-  signature eqv ==> eqv ==> iff as le_mor.
-Proof.
-  intros.
-  unfold eqv in *. intuition; eauto using le_trans.
-Qed.
-
-Add Parametric Morphism {A} `{Ord A} : lt with
-  signature eqv ==> eqv ==> iff as lt_mor.
-Proof.
-  intros.
-  unfold eqv, lt in *. intuition; eauto using le_trans.
-Qed.
+  Global Instance Ord_EquivDef {A} `{Ord A} : EqDec A eq.
+  Proof.
+    intros x y.
+    destruct (eqv_dec x y).
+    - left. apply eqv_eq. auto.
+    - right. intro c. apply n. rewrite c. reflexivity.
+  Defined.
+End Ord.
